separate boundary condition from the invariants

ironfleet/src/Dafny/Distributed/Protocol/RSL/FailureProof/Phase2Proof_postFail.i.dfy
@@ -80,8 +80,6 @@ predicate RslAssumption(s:TimestampedRslState)
 
 predicate RelationsAssumptions() {
     && TimeLe(req_time, NewLeaderInitTS)
-    && TimeLe(Old_1aTS + MaxQueueTime + ProcessPacket + D, Old_1bTS)
-    && TimeLe(Old_2aTS + MaxQueueTime + ProcessPacket + TimeActionRange(0) + D, Old_2bTS)
 }
 
 predicate LeaderAlwaysOne(s:TimestampedRslState) 
@@ -136,76 +134,45 @@ predicate RequestBatchSrcInClientIds(s:TimestampedRslState, v:RequestBatch)
     forall r :: r in v ==> r.client in s.constants.config.clientIds
 }
 
+
 /*****************************************************************************************
-*                                     Invariants                                        *
+*                                    Boundary State                                      *
 *****************************************************************************************/
 
 /* Timestamp of initial client request */
 ghost const req_time:Timestamp
-/* Timestamps of stale packets */
-ghost const Old_2aTS:Timestamp
-ghost const Old_2bTS:Timestamp
-ghost const Old_1aTS:Timestamp
-ghost const Old_1bTS:Timestamp
 /* Initial timestamp of replica 1 */
 ghost const NewLeaderInitTS:Timestamp
 
-
-predicate RslPerfInvariant(s:TimestampedRslState, req_time:Timestamp, opn:OperationNumber) 
-    requires |s.t_replicas| > 2
-{
-    && RslConsistency(s)
-    && BoundaryConditionInvariant(s)
-    && PerformanceGuarantee(s)
-}
-
-
 //  Invariant of starting state of Phase2 proof
-predicate BoundaryConditionInvariant(s:TimestampedRslState) 
+predicate BoundaryCondition(s:TimestampedRslState) 
     requires |s.t_replicas| > 2
 {
-    && BoundaryConditionInvariant_ExistingPacketsBallot(s)
-    && BoundaryConditionInvariant_ExistingPacketsTS(s)
-    // && BoundaryConditionInvariant_NewLeader(s)
+    && BoundaryCondition_ExistingPacketsBallot(s)
+    && BoundaryCondition_NewLeader(s)
 }
 
-predicate BoundaryConditionInvariant_ExistingPacketsTS(s:TimestampedRslState) {
-    forall pkt | pkt in s.undeliveredPackets :: Boundary_ExistingPacketsTS(pkt)
+
+predicate BoundaryCondition_NewLeader(s:TimestampedRslState) {
+    // TODO
+    true
 }
 
-predicate BoundaryConditionInvariant_ExistingPacketsBallot(s:TimestampedRslState) {
+
+predicate BoundaryCondition_ExistingPacketsBallot(s:TimestampedRslState) {
     forall pkt | pkt in s.undeliveredPackets :: Boundary_ExistingPacketsBallot(pkt)
 }
-
-predicate Boundary_ExistingPacketsTS(pkt:TimestampedLPacket<EndPoint, RslMessage>) {
-    match pkt.msg.v {
-        case RslMessage_1a(_)               => TimeLe(pkt.msg.ts, Old_1aTS) 
-        case RslMessage_1b(_,_,_)           => TimeLe(pkt.msg.ts, Old_1bTS) 
-        case RslMessage_2a(bal_2a,_,_)      => bal_2a == Ballot(1, 0)  ==> TimeLe(pkt.msg.ts, Old_2aTS) 
-        case RslMessage_2b(bal_2b,_,_)      => bal_2b == Ballot(1, 0)  ==> TimeLe(pkt.msg.ts, Old_2bTS) 
-        case RslMessage_Request(_,_)        => TimeLe(pkt.msg.ts, req_time) 
-
-        // Cases where I don't care
-        case RslMessage_Heartbeat(_,_,_)        => true
-        case RslMessage_Invalid                 => true
-        case RslMessage_Reply(_,_)              => true
-        case RslMessage_AppStateRequest(_,_)    => true
-        case RslMessage_AppStateSupply(_,_,_,_) => true
-        case RslMessage_StartingPhase2(_,_)     => true
-    }
-}
-
 predicate Boundary_ExistingPacketsBallot(pkt:TimestampedLPacket<EndPoint, RslMessage>) {
     match pkt.msg.v {
         // All 1a and 1b packets have Ballot (1, 1)
         case RslMessage_1a(bal_1a)              => bal_1a == Ballot(1, 1) 
         case RslMessage_1b(bal_1b,_,_)          => bal_1b == Ballot(1, 1) 
-        // All 2a and 2b messages have Ballot(1, 0) or (1, 1)
-        case RslMessage_2a(bal_2a,_,_)          => bal_2a == Ballot(1, 0) || bal_2a == Ballot(1, 1)
-        case RslMessage_2b(bal_2b,_,_)          => bal_2b == Ballot(1, 0) || bal_2b == Ballot(1, 1)
+        // All 2a and 2b messages have Ballot(1, 0)
+        case RslMessage_2a(bal_2a,_,_)          => bal_2a == Ballot(1, 0)
+        case RslMessage_2b(bal_2b,_,_)          => bal_2b == Ballot(1, 0)
 
         // Cases where I don't care
-        case RslMessage_Heartbeat(_,_,_)   => true
+        case RslMessage_Heartbeat(_,_,_)        => true
         case RslMessage_Invalid                 => true
         case RslMessage_Request(_,_)            => true
         case RslMessage_Reply(_,_)              => true
@@ -216,10 +183,44 @@ predicate Boundary_ExistingPacketsBallot(pkt:TimestampedLPacket<EndPoint, RslMes
 }
 
 
-predicate LeaderYetReceived2b(s:TimestampedRslState) 
+
+
+
+/*****************************************************************************************
+*                                     Invariants                                        *
+*****************************************************************************************/
+
+
+// Main invariant 
+predicate RslPerfInvariant(s:TimestampedRslState, req_time:Timestamp, opn:OperationNumber) 
     requires |s.t_replicas| > 2
 {
-    s.t_replicas[1].v.replica.proposer.received_1b_packets == {}
+    && RslConsistency(s)
+    && PerformanceGuarantee(s)
+    && PacketsBallotInvariant(s)
 }
 
+predicate PacketsBallotInvariant(s:TimestampedRslState) {
+    forall pkt | pkt in s.undeliveredPackets :: ExistingPacketsBallot(pkt)
+}
+
+predicate ExistingPacketsBallot(pkt:TimestampedLPacket<EndPoint, RslMessage>) {
+    match pkt.msg.v {
+        // All 1a and 1b packets have Ballot (1, 1)
+        case RslMessage_1a(bal_1a)              => bal_1a == Ballot(1, 1) 
+        case RslMessage_1b(bal_1b,_,_)          => bal_1b == Ballot(1, 1) 
+        // All 2a and 2b messages have Ballot(1, 0) or (1, 1)
+        case RslMessage_2a(bal_2a,_,_)          => bal_2a == Ballot(1, 0) || bal_2a == Ballot(1, 1)
+        case RslMessage_2b(bal_2b,_,_)          => bal_2b == Ballot(1, 0) || bal_2b == Ballot(1, 1)
+
+        // Cases where I don't care
+        case RslMessage_Heartbeat(_,_,_)        => true
+        case RslMessage_Invalid                 => true
+        case RslMessage_Request(_,_)            => true
+        case RslMessage_Reply(_,_)              => true
+        case RslMessage_AppStateRequest(_,_)    => true
+        case RslMessage_AppStateSupply(_,_,_,_) => true
+        case RslMessage_StartingPhase2(_,_)     => true
+    }
+}
 }
