ironfleet/src/Dafny/Distributed/Protocol/RSL/FailureProof/Phase2Proof_postFail_helper.i.dfy
@@ -5,115 +5,24 @@ import opened RslPhase2Proof_postFail_i
 
 
 /* Note: this requires a long timeout to verify */
-lemma BoundaryInvariantsMaintained_ReceiveStep_ExistingPacketsBallot(ts:TimestampedRslState, ts':TimestampedRslState, req_time:Timestamp, opn:OperationNumber, idx:int, tios:seq<TimestampedLIoOp<NodeIdentity, RslMessage>>) 
+lemma PacketsBallotInvariant_ReceiveStep(ts:TimestampedRslState, ts':TimestampedRslState, req_time:Timestamp, opn:OperationNumber, idx:int, tios:seq<TimestampedLIoOp<NodeIdentity, RslMessage>>) 
     requires RslAssumption(ts) && RslConsistency(ts)
     requires RslAssumption(ts') && RslConsistency(ts')
     requires TimestampedRslNext(ts, ts')
     requires RslPerfInvariant(ts, req_time, opn)
     requires TimestampedRslNextOneReplica(ts, ts', idx, tios);
     requires ts.t_replicas[idx].v.nextActionIndex == 0 
-    ensures BoundaryConditionInvariant_ExistingPacketsBallot(ts')
-{
-    var tsSentPackets := (set io | io in tios && io.LIoOpSend? :: io.s);
-    var s, s', ios := UntimestampRslState(ts), UntimestampRslState(ts'), UntagLIoOpSeq(tios);
-    var r, r' := s.replicas[idx].replica, s'.replicas[idx].replica;
+    ensures PacketsBallotInvariant(ts')
+{}
 
-    if ios[0].LIoOpTimeoutReceive? {
-        return;
-    }
-    if ios[0].r.msg.RslMessage_Heartbeat? {
-        assert false;
-    } else {
-        var sentPackets := ExtractSentPacketsFromIos(ios);
-        match ios[0].r.msg {
-            case RslMessage_Invalid => assert true;
-            case RslMessage_Request(_, _) => 
-                forall pkt | pkt in ts'.undeliveredPackets 
-                ensures Boundary_ExistingPacketsBallot(pkt)
-                {
-                    if pkt !in ts.undeliveredPackets {
-                        assert pkt in tsSentPackets;
-                        assert pkt.msg.v.RslMessage_Reply?;
-                    }
-                }                
-            case RslMessage_1a(_) => 
-                forall pkt | pkt in ts'.undeliveredPackets 
-                ensures Boundary_ExistingPacketsBallot(pkt)
-                {}
-            case RslMessage_1b(_, _, _) => assert true;
-            case RslMessage_StartingPhase2(_, _) =>
-                assert forall pkt | pkt in tsSentPackets :: pkt.msg.v.RslMessage_AppStateRequest?;
-                forall pkt | pkt in ts'.undeliveredPackets 
-                ensures Boundary_ExistingPacketsBallot(pkt)
-                {
-                    if pkt !in ts.undeliveredPackets {
-                        assert pkt in tsSentPackets;
-                        assert pkt.msg.v.RslMessage_AppStateRequest?;
-                    }
-                }
-            case RslMessage_2a(_, _, _) => 
-                forall pkt | pkt in ts'.undeliveredPackets 
-                ensures Boundary_ExistingPacketsBallot(pkt)
-                {}
-            case RslMessage_2b(_, _, _) => assert true;
-            case RslMessage_Reply(_, _) => assert true;
-            case RslMessage_AppStateRequest(_, _) => 
-                forall pkt | pkt in ts'.undeliveredPackets 
-                ensures Boundary_ExistingPacketsBallot(pkt)
-                {
-                    if pkt !in ts.undeliveredPackets {
-                        assert pkt in tsSentPackets;
-                        assert pkt.msg.v.RslMessage_AppStateSupply?;
-                    }
-                }                
-            case RslMessage_AppStateSupply(_, _, _, _) => assert true;               
-        }
-         
-    }
-}
-
-
-lemma BoundaryInvariantsMaintained_ReceiveStep_ExistingPacketsTS(ts:TimestampedRslState, ts':TimestampedRslState, req_time:Timestamp, opn:OperationNumber, idx:int, tios:seq<TimestampedLIoOp<NodeIdentity, RslMessage>>) 
-    requires RslAssumption(ts) && RslConsistency(ts)
-    requires RslAssumption(ts') && RslConsistency(ts')
-    requires TimestampedRslNext(ts, ts')
-    requires RslPerfInvariant(ts, req_time, opn)
-    requires TimestampedRslNextOneReplica(ts, ts', idx, tios);
-    requires ts.t_replicas[idx].v.nextActionIndex == 0 
-    ensures BoundaryConditionInvariant_ExistingPacketsTS(ts')
-{
-    // var tsSentPackets := (set io | io in tios && io.LIoOpSend? :: io.s);
-    var s, s', ios := UntimestampRslState(ts), UntimestampRslState(ts'), UntagLIoOpSeq(tios);
-    // var r, r' := s.replicas[idx].replica, s'.replicas[idx].replica;
-
-    if ios[0].LIoOpTimeoutReceive? {
-        return;
-    }
-    if ios[0].r.msg.RslMessage_Heartbeat? {
-        assert false;
-    }
-}
-
-lemma BoundaryInvariantsMaintained_NoReceiveStep_ExistingPacketsBallot(ts:TimestampedRslState, ts':TimestampedRslState, req_time:Timestamp, opn:OperationNumber, idx:int, tios:seq<TimestampedLIoOp<NodeIdentity, RslMessage>>) 
+lemma PacketsBallotInvariant_NoReceiveStep(ts:TimestampedRslState, ts':TimestampedRslState, req_time:Timestamp, opn:OperationNumber, idx:int, tios:seq<TimestampedLIoOp<NodeIdentity, RslMessage>>) 
     requires RslAssumption(ts) && RslConsistency(ts)
     requires RslAssumption(ts') && RslConsistency(ts')
     requires TimestampedRslNext(ts, ts')
     requires RslPerfInvariant(ts, req_time, opn)
     requires TimestampedRslNextOneReplica(ts, ts', idx, tios);
     requires ts.t_replicas[idx].v.nextActionIndex != 0 
-    ensures BoundaryConditionInvariant_ExistingPacketsBallot(ts')
-{
-    assert BoundaryConditionInvariant_ExistingPacketsBallot(ts');
-}
-
-lemma BoundaryInvariantsMaintained_NoReceiveStep_ExistingPacketsTS(ts:TimestampedRslState, ts':TimestampedRslState, req_time:Timestamp, opn:OperationNumber, idx:int, tios:seq<TimestampedLIoOp<NodeIdentity, RslMessage>>) 
-    requires RslAssumption(ts) && RslConsistency(ts)
-    requires RslAssumption(ts') && RslConsistency(ts')
-    requires TimestampedRslNext(ts, ts')
-    requires RslPerfInvariant(ts, req_time, opn)
-    requires TimestampedRslNextOneReplica(ts, ts', idx, tios);
-    requires ts.t_replicas[idx].v.nextActionIndex != 0 
-    ensures BoundaryConditionInvariant_ExistingPacketsTS(ts')
+    ensures PacketsBallotInvariant(ts')
 {}
 
 }
